Fixe Definitionen von computes* und Komposition

TM/CodeTM.v
@@ -1,6 +1,6 @@
 Require Import Prelim TM LiftNM LiftSigmaTau Code.
 (* Require Import Basic.Mono Compound. *)
-Require Import Combinators.If Combinators.While.
+Require Import Combinators.If Combinators.While Combinators.SequentialComposition.
 Require Import TM.Relations.
 
 Definition bool_fin : finType := FinType (EqType bool).
@@ -20,6 +20,10 @@ Section Tape_Local.
     tape_local t = x :: xs -> current t = Some x.
   Proof. destruct t eqn:E; cbn; try congruence. Qed.
 
+  Lemma tape_local_right (x : sig) (xs : list sig) (t : tape sig) :
+    tape_local t = x :: xs -> right t = xs.
+  Proof. destruct t eqn:E; cbn; try congruence. Qed.
+    
 End Tape_Local.
     
 Section Tape_Encodes.
@@ -93,47 +97,99 @@ Section Computes.
 
   Definition computes_locally_R : relation (tapes bool_fin n_tapes) :=
     fun tin tout =>
-      forall (x : X) (y : Y),
+      forall (x : X),
         tape_encodes_locally _ ( tin[@i]) x ->
-        tape_encodes_locally _ (tout[@j]) y ->
-        f x = y.
+        tape_encodes_locally _ (tout[@j]) (f x).
 
   Definition computes_locally_R' : relation (tapes bool_fin n_tapes) :=
     fun tin tout =>
-      forall (x : X) (y : Y),
+      forall (x : X),
         tape_encodes_locally' _ ( tin[@i]) x ->
-        tape_encodes_locally' _ (tout[@j]) y ->
-        f x = y.
+        tape_encodes_locally' _ (tout[@j]) (f x).
 
   Lemma computes_locally_R_iff (tin tout : tapes bool_fin n_tapes) :
     computes_locally_R tin tout <-> computes_locally_R' tin tout.
-  Proof. unfold computes_locally_R, computes_locally_R'; intuition; apply H; now rewrite tape_encodes_locally_iff in *. Qed.
+  Proof.
+    unfold computes_locally_R, computes_locally_R'; intuition.
+    rewrite <- tape_encodes_locally_iff in *; auto.
+    rewrite -> tape_encodes_locally_iff in *; auto.
+  Qed.
 
   Definition computes_locally_R_p : Rel (tapes bool_fin n_tapes) (F * tapes bool_fin n_tapes) :=
     ignoreParam (computes_locally_R).
 
   Definition computes_global_R : relation (tapes bool_fin n_tapes) :=
     fun tin tout =>
-      forall (x : X) (y : Y),
+      forall (x : X),
         tape_encodes_global _ ( tin[@i]) x ->
-        tape_encodes_global _ (tout[@j]) y ->
-        f x = y.
+        tape_encodes_global _ (tout[@j]) (f x).
   
   Definition computes_global_R' : relation (tapes bool_fin n_tapes) :=
     fun tin tout =>
-      forall (x : X) (y : Y),
+      forall (x : X),
         tape_encodes_global' _ ( tin[@i]) x ->
-        tape_encodes_global' _ (tout[@j]) y ->
-        f x = y.
+        tape_encodes_global' _ (tout[@j]) (f x).
 
   Lemma computes_global_R_iff (tin tout : tapes bool_fin n_tapes) :
     computes_global_R tin tout <-> computes_global_R' tin tout.
-  Proof. unfold computes_global_R, computes_global_R'; intuition; apply H; now rewrite tape_encodes_global_iff in *. Qed.
+  Proof.
+    unfold computes_global_R, computes_global_R'; intuition.
+    rewrite <- tape_encodes_global_iff in *; auto.
+    rewrite -> tape_encodes_global_iff in *; auto.
+  Qed.
 
   Definition computes_global_R_p : Rel (tapes bool_fin n_tapes) (F * tapes bool_fin n_tapes) :=
     ignoreParam (computes_global_R).
 
 End Computes.
+
+Section Computes_Composes.
+
+  Variable (X Y Z : Type) (cX : codeable X) (cY : codeable Y) (cZ : codeable Z).
+  Variable (f : X -> Y) (g : Y -> Z).
+  Variable (n_tapes : nat).
+  Variable (i1 i2 i3 : Fin.t (S n_tapes)).
+  Variable (F1 F2 : finType).
+  Variable (pM : {M : mTM bool_fin n_tapes & states M -> F1}).
+  Variable (pN : {N : mTM bool_fin n_tapes & states N -> F2}).
+
+  Lemma compose_computes_sem (iin iout : Fin.t (S n_tapes)) :
+    pM ⊫ computes_locally_R_p (F := F1) i1 i2 _ _ f ->
+    pN ⊫ computes_locally_R_p (F := F2) i2 i3 _ _ g ->
+    (pM ;; pN) ⊫ computes_locally_R_p (F := F2) i1 i3 _ _ (fun x => g (f x)).
+  Proof.
+    intros H1 H2.
+    pose proof (SequentialComposition.Seq_sem H1 H2) as HComp.
+    hnf. intros intape i outc HLoop.
+    hnf. intros x Hx. cbn in outc.
+    specialize (HComp intape i outc HLoop).
+    unfold rcomp in HComp.
+    destruct HComp as ((exectape_p&exectape)&HComp&HComp'); cbn in HComp, HComp'.
+    unfold computes_locally_R in *.
+    apply HComp'. apply HComp. assumption.
+  Qed.
+
+  Print SequentialComposition.
+
+  Lemma compose_computes_total (iin iout : Fin.t (S n_tapes)) (k1 k2 : nat) :
+    pM ⊨(k1) computes_locally_R_p (F := F1) i1 i2 _ _ f ->
+    pN ⊨(k2) computes_locally_R_p (F := F2) i2 i3 _ _ g ->
+    (pM ;; pN) ⊨(1+k1+k2) computes_locally_R_p (F := F2) i1 i3 _ _ (fun x => g (f x)).
+  Proof.
+    intros H1 H2.
+    pose proof (SequentialComposition.Seq_total H1 H2) as HComp.
+    intros intape.
+    specialize (HComp intape) as (outtape&HLoop&HComp).
+    unfold computes_locally_R_p in HComp. cbn in HComp.
+    unfold rcomp in HComp.
+    destruct HComp as ((exectape_p&exectape)&HComp&HComp'); cbn in HComp, HComp'.
+    unfold computes_locally_R in *. clear exectape_p.
+    exists outtape. split.
+    - apply HLoop.
+    - cbn. hnf. intros x Hx. apply HComp'. apply HComp. apply Hx.
+  Qed.
+
+End Computes_Composes.
 
 
 Section Neg_TM.
@@ -187,12 +243,12 @@ Section Neg_TM.
     unfold loopM in *.
     erewrite (loop_ge (k1 := 1) (k2 := i)) in HLoop. Focus 2. omega. Focus 2.
     cbn. unfold id. unfold neg_TM. cbn. rewrite neg_TM_onestep. reflexivity. inv HLoop.
-    apply computes_locally_R_iff. hnf. intros x y (rest1&E1) (rest2&E2).
+    apply computes_locally_R_iff. hnf. intros x (rest1&E1).
     unfold initc, step, neg_TM in *. cbn in *.
     dependent induction inittapes. dependent induction inittapes. cbn in *. clear IHinittapes.
-    dependent induction outt. dependent induction outt. cbn in *. clear IHoutt.
-    destruct x, y; cbn in *;
-      erewrite !tape_local_current_cons in H1; eauto; cbn in *; inv H1; cbn in *; congruence.
+    hnf.
+    destruct x; cbn in *;
+      erewrite !tape_local_current_cons in H1; eauto; cbn in *; inv H1; cbn in *; now eauto.
   Qed.
 
   Lemma neg_TM_computes_terminates_in :
@@ -200,5 +256,18 @@ Section Neg_TM.
   Proof.
     hnf. intros inittape i ->. cbn. unfold id. rewrite neg_TM_onestep. eauto.
   Qed.
+
+  Lemma neq_TM_computes_total :
+    neg_mTM ⊨(1) computes_locally_R_p (F := F) Fin.F1 Fin.F1 _ _ negb.
+  Proof.
+    hnf. intros inittape.
+    dependent induction inittape. dependent induction inittape. clear IHinittape; cbn in *.
+    unfold id. rewrite neg_TM_onestep. econstructor. split. eauto.
+    hnf. intros x.
+    rewrite !tape_encodes_locally_iff. unfold tape_encodes_locally'. intros (tape&bl). cbn in *.
+    destruct x; cbn in *; exists tape;
+      cbn; unfold neg_TM, step; cbn;
+        erewrite tape_local_current_cons; eauto; cbn; f_equal; eapply tape_local_right; eauto.
+    Qed.
   
 End Neg_TM.
